src/probability/util_probScript.sml
@@ -10,11 +10,9 @@
 open HolKernel Parse boolLib bossLib;
 
 open metisLib pairTheory combinTheory pred_setTheory pred_setLib jrhUtils
-     arithmeticTheory numLib numpairTheory hurdUtils whileTheory;
+     arithmeticTheory numLib hurdUtils;
 
-open realTheory realLib transcTheory seqTheory real_sigmaTheory RealArith;
-
-open topologyTheory iterateTheory;
+open realTheory realLib real_sigmaTheory iterateTheory;
 
 val _ = new_theory "util_prob";
 
@@ -39,12 +37,6 @@ val _ = TeX_notation {hol = "->",            TeX = ("\\HOLTokenMap{}", 1)};
 val _ = TeX_notation {hol = UTF8.chr 0x2192, TeX = ("\\HOLTokenMap{}", 1)};
 val _ = TeX_notation {hol = "-->",           TeX = ("\\HOLTokenLongmap{}", 1)};
 val _ = TeX_notation {hol = UTF8.chr 0x27F6, TeX = ("\\HOLTokenLongmap{}", 1)};
-
-Theorem IN_o :
-    !x f s. x IN (s o f) <=> f x IN s
-Proof
-    RW_TAC std_ss [SPECIFICATION, o_THM]
-QED
 
 Definition prod_sets_def :
     prod_sets a b = {s CROSS t | s IN a /\ t IN b}
